Fixing the counter protocol (progress)

contrib/Platform/ml/platform.ml
@@ -112,6 +112,7 @@ let split (b:bytes) i : bytes * bytes =
      length = b.length - i;
      index = b.index + i;
      max = b.max}
+let split_eq = split
 let length (d:bytes) = d.length
 
 
