contrib/Platform/fst/Bytes.fst
@@ -101,6 +101,20 @@ val split: b:bytes -> n:nat{n <= Seq.length b} -> Tot (x:(bytes * bytes) {Seq.le
 let split b n =
   SeqProperties.split b n
 
+val lemma_split : #a:Type -> s:bytes -> i:nat{(0 <= i /\ i <= length s)} -> Lemma
+  (ensures ((fst (split s i)) @| (snd (split s i)) = s))
+let lemma_split s i =
+  cut (Seq.Eq ((fst (split s i)) @| (snd (split s i)))  s)
+
+val split_eq: #a:Type -> s:bytes -> i:nat{(0 <= i /\ i <= length s)} -> Pure
+  (x:(bytes * bytes){length (fst x) = i && length (snd x) = length s - i})
+  (requires True)
+  (ensures (fun x -> ((fst x) @| (snd x) = s)))
+let split_eq s i =
+  let x = split s i in
+  lemma_split s i;
+  x
+
 (*@ assume val split2 : (b:bytes -> (i:nat -> ((j:nat){C_pr_GreaterThanOrEqual(Length (b), C_bop_Addition (i, j))} -> (b1:bytes * b2:bytes * b3:bytes){Length (b1) = i /\ Length (b2) = j /\ B (b) = C_bop_ArrayAppend (B (b1), C_bop_ArrayAppend (B (b2), B (b3)))}))) @*)
 assume val split2 : b:bytes -> n1:nat{n1 <= Seq.length b} -> n2:nat{n1 + n2 <= Seq.length b} -> Tot (lbytes n1 * lbytes n2 * lbytes (length b - n1 - n2))
 (*@  assume (!x. C_bop_ArrayAppend (x, C_array_of_list C_op_Nil ()) = x) @*)
